\documentclass{article}
\input{503macros.tex}
\usepackage{stmaryrd}

\def\Sometime{\mathord{\mathsf{F}}}
\def\Forever{\mathord{\mathsf{G}}}
\def\Next{\mathord{\mathsf{O}}}
\def\NextX{\mathord{\mathsf{X}}}
\def\Until{\mathrel{\mathsf{U}}}
\def\Release{\mathrel{\mathsf{R}}}
\def\WeakUntil{\mathrel{\mathsf{W}}}
\def\Before{\mathrel{\mathsf{B}}}
\def\True{\mathord{\mathsf{true}}}
\def\All{\mathord{\mathsf{A}}}
\def\Exists{\mathord{\mathsf{E}}}
\def\Every{\mathord{\mathsf{E}}}

\def\True{\mathord{\mathtt{true}}}
\def\False{\mathord{\mathtt{false}}}
\def\If{\mathrel{\mathtt{if}}}
\def\Else{\mathrel{\mathtt{else}}}
\def\While{\mathrel{\mathtt{while}}}
\def\IfElse#1#2#3{\If #1 \ \{ #2 \} \Else \{ #3 \}}
\def\Whiledo#1#2{\While #1\ \{ #2 \}}
\def\Hcond#1{\llparenthesis #1 \rrparenthesis}
\def\Hoare#1#2#3{\Hcond{#1} \mathrel{#2} \Hcond{#3}}

\def\parmodels{\mathrel{\models_{\textup{par}}}}
\def\totmodels{\mathrel{\models_{\textup{tot}}}}
\def\parturn{\mathrel{\turn_{\textup{par}}}}
\def\totturn{\mathrel{\turn_{\textup{tot}}}}

\title{CSC 503 Homework Assignment 12}
\author{Due November 17, 2014}
\date{November 10, 2014}

\begin{document}
\maketitle

\begin{enumerate}

\item {[100 points]} Find a natural deduction proof in the basic modal
  logic K for the formula
  \begin{displaymath}
    (K (p \implies q)) \implies (\neg K \neg p \implies \neg K \neg q).
  \end{displaymath}
  Use the justifications \verb+\Ki+ and \verb+\Ke+ for the respective
  modal inference rules, and \verb+\open[K]+ to introduce a modal
  context.  You may use derived rules of inference, including Modus
  Tollens (\verb+\mt+).
	\begin{answer}
		\[
			\begin{nd}
				\open
					\hypo{1} {K (p \implies q)} \assumption{}
					\open
						\hypo{2} {\neg K \neg p} \assumption{}
						\open
							\hypo{3} {K \neg q} \assumption{}
							\open[K] 
								\have{4} {p \implies q} \Ke {1}
								\have{5} {\neg q} \Ke {3}
								\have{6} {\neg p} \mt {4, 5}
							\close
							\have{7} {K \neg p} \Ki {4-6}
							\have{8} {\bot} \ne {2, 7}
						\close
						\have{9} {\neg K \neg q} \ni {3, 8}
					\close
					\have{10} {\neg K \neg p \implies \neg K \neg q} \ii {2, 9}
				\close
				\have{11} {( K (p \implies q)) \implies (\neg K \neg p \implies \neg K \neg
				q)} \ii {1, 10}
			\end{nd}
		\]
	\end{answer}
\end{enumerate}
\end{document}
