\documentclass{article}
\input{503macros.tex}
\usepackage{stmaryrd}

\def\Sometime{\mathord{\mathsf{F}}}
\def\Forever{\mathord{\mathsf{G}}}
\def\Next{\mathord{\mathsf{O}}}
\def\NextX{\mathord{\mathsf{X}}}
\def\Until{\mathrel{\mathsf{U}}}
\def\Release{\mathrel{\mathsf{R}}}
\def\WeakUntil{\mathrel{\mathsf{W}}}
\def\Before{\mathrel{\mathsf{B}}}
\def\True{\mathord{\mathsf{true}}}
\def\All{\mathord{\mathsf{A}}}
\def\Exists{\mathord{\mathsf{E}}}
\def\Every{\mathord{\mathsf{E}}}

\def\True{\mathord{\mathtt{true}}}
\def\False{\mathord{\mathtt{false}}}
\def\If{\mathrel{\mathtt{if}}}
\def\Else{\mathrel{\mathtt{else}}}
\def\While{\mathrel{\mathtt{while}}}
\def\IfElse#1#2#3{\If #1 \ \{ #2 \} \Else \{ #3 \}}
\def\Whiledo#1#2{\While #1\ \{ #2 \}}
\def\Hcond#1{\llparenthesis #1 \rrparenthesis}
\def\Hoare#1#2#3{\Hcond{#1} \mathrel{#2} \Hcond{#3}}

\def\parmodels{\mathrel{\models_{\textup{par}}}}
\def\totmodels{\mathrel{\models_{\textup{tot}}}}
\def\parturn{\mathrel{\turn_{\textup{par}}}}
\def\totturn{\mathrel{\turn_{\textup{tot}}}}

\title{CSC 503 Homework Assignment 11}
\author{Due November 12, 2014}
\date{November 5, 2014}

\begin{document}
\maketitle

\begin{enumerate}

\item {[100 points]} Show that $\parturn \Hoare{y = y_0 \land y \ge 0}{\hbox{Multi2}}{z = x \cdot y_0}$ is valid, where Multi2 is the
  program
  \begin{displaymath}
    \begin{nd}
      \have{} {\texttt{\textbf{z = 0;}}}   
      \have{} {\texttt{\textbf{while (y != 0) \{}}}          
      \have{} {\quad\texttt{\textbf{z = z + x;}}}                   
      \have{} {\quad\texttt{\textbf{y = y - 1;}}}                   
      \have{} {\texttt{\textbf{\}}}}                  
    \end{nd}
  \end{displaymath}
\begin{answer}
	\begin{displaymath}
    \begin{nd}
      \have{} {\Hcond{y = y_0 \land y \ge 0}} 
      \have{} {\Hcond{0 = x \cdot (y_0 - y)}} \Implied{}
      \have{} {\texttt{\textbf{z = 0;}}}   
      \have{} {\Hcond{z = x \cdot (y_0 - y)}} \Assignment{}
      \have{} {\texttt{\textbf{while (y != 0) \{}}}
      \have{} {\Hcond{z = x \cdot (y_0 - y) \land (y != 0)}} \InvariantGuard{}
      \have{} {\Hcond{z + x = x \cdot (y_0 - (y - 1))}} \Implied{}         
      \have{} {\quad\texttt{\textbf{z = z + x;}}}          
      \have{} {\Hcond{z = x \cdot (y_0 - (y - 1))}} \Assignment{}         
      \have{} {\quad\texttt{\textbf{y = y - 1;}}}                   
      \have{} {\Hcond{z = x \cdot (y_0 - y)}} \Assignment{}
      \have{} {\texttt{\textbf{\}}}}
      \have{} {\Hcond{z = x \cdot (y_0 - y) \land \neg (y != 0)}} \PartialWhile{}
      \have{} {\Hcond{z = x \cdot y_0}} \Implied{}
    \end{nd}
  \end{displaymath}
\end{answer}
\end{enumerate}
\end{document}
